new/golang/defn/array.v
@@ -1,0 +1,50 @@
+From New.golang.defn Require Export predeclared.
+
+Module go.
+Section defs.
+Context `{ffi_syntax}.
+
+Class ArraySemantics {go_ctx : GoContext} :=
+{
+  equals_array n t V (a1 a2 : array.t t V n) `{!EqDecision V} `{!IntoVal V}
+    (H : go.is_strictly_comparable t V) :
+    go.is_strictly_comparable (go.ArrayType n t) (array.t t V n);
+
+  alloc_array n elem : alloc (go.ArrayType n elem) = alloc (go.ArrayType n elem); (* TODO *)
+  load_array n elem_type :
+    load (go.ArrayType n elem_type) =
+    if decide (¬(0 ≤ n < 2^63-1)) then
+      (λ: "l", AngelicExit #())%V
+        (* the compiler guarantees that any compiled code does not have an array this size *)
+    else
+      (λ: "l",
+         (rec: "recur" "n" :=
+            if: "n" =⟨go.int⟩ #(W64 0) then (ArrayV [])
+            else let: "array_so_far" := "recur" ("n" - #(W64 1)) in
+                 let: "elem_addr" := IndexRef (go.ArrayType n elem_type) ("l", "n" - #(W64 1)) in
+                 let: "elem_val" := GoLoad elem_type "elem_addr" in
+                 ArrayAppend ("array_so_far", "elem_val")
+         ) #(W64 n))%V;
+  store_array n elem_type :
+    store (go.ArrayType n elem_type) =
+    (λ: "l" "v",
+       foldl (λ str_so_far j,
+                str_so_far;;
+                let elem_addr := IndexRef (go.ArrayType n elem_type) ("l", #(W64 j)) in
+                let elem_val := Index (go.ArrayType n elem_type) ("v", #(W64 n)) in
+                GoStore elem_type (elem_addr, elem_val))
+             (ArrayV []) (seqZ 0 n)
+    )%V;
+
+
+  index_ref_array n elem_type i l :
+    index_ref (go.ArrayType n elem_type) i #l = #(array_index_ref elem_type i l);
+  index_array n elem_type i l v (Hinrange : l !! (Z.to_nat i) = Some v):
+    index (go.ArrayType n elem_type) i (ArrayV l) = (Val v);
+
+  array_index_ref_add t i j l :
+    array_index_ref t (i + j) l = array_index_ref t j (array_index_ref t i l);
+}.
+
+End defs.
+End go.
