new/golang/theory/exception.v
@@ -1,17 +1,15 @@
 From New.golang.defn Require Export exception.
 From New.golang.theory Require Export predeclared.
-From iris.proofmode Require Import coq_tactics.
-Import Ltac2.
-Set Default Proof Mode "Classic".
 
 Section wps.
-Context `{sem: ffi_semantics} `{!ffi_interp ffi} `{!heapGS Σ}.
+Context `{sem: ffi_semantics} `{!ffi_interp ffi} `{!heapGS Σ}
+  {core_sem : go.CoreSemantics} {pre_sem : go.PredeclaredSemantics}.
 
 Global Instance pure_execute_val (v : val) :
   PureWp True (exception_seq v (execute_val)) (v #()).
 Proof.
   rewrite exception_seq_unseal execute_val_unseal.
-  intros ?????. iIntros "Hwp". wp_call_lc "?". rewrite bool_decide_true //.
+  intros ?????. iIntros "Hwp". wp_call_lc "?".
   wp_pures. by iApply "Hwp".
 Qed.
 
@@ -27,7 +25,7 @@ Global Instance pure_return_val (v1 : val) (v : val) :
 Proof.
   rewrite exception_seq_unseal return_val_unseal.
   intros ?????. iIntros "Hwp".
-  wp_call_lc "?". rewrite bool_decide_false //. wp_pures. by iApply "Hwp".
+  wp_call_lc "?". wp_pures. by iApply "Hwp".
 Qed.
 
 Global Instance pure_do_return_val (v : val) : PureWp True (return: v) (return_val v).
