new/golang/theory/predeclared.v
@@ -10,7 +10,7 @@ End error.
 
 Section into_val_typed_instances.
 Context `{ffi_sem: ffi_semantics} `{!ffi_interp ffi} `{!heapGS Σ}
-  {Hcore : go.CoreSemantics} {Hpredeclared : go.PredeclaredSemantics}.
+  {core_sem : go.CoreSemantics} {pre_sem : go.PredeclaredSemantics}.
 
 Ltac solve_wp_alloc :=
   iIntros "* _ HΦ";
@@ -38,51 +38,210 @@ Existing Class go.is_predeclared.
 Existing Class go.is_predeclared_zero_val.
 #[local] Hint Extern 1 (go.is_predeclared_zero_val ?t ?v) => constructor : typeclass_instances.
 
+Local Set Default Proof Using "Type core_sem pre_sem".
 Global Instance into_val_typed_uint64 : IntoValTyped w64 go.uint64.
-Proof using Hpredeclared. solve_into_val_typed. Qed.
+Proof. solve_into_val_typed. Qed.
+Global Instance into_val_comparable_uint64 : IntoValComparable w64 go.uint64.
+Proof. constructor. apply go.comparable_ordered. repeat constructor. Qed.
 
 Global Instance into_val_typed_uint32 : IntoValTyped w32 go.uint32.
-Proof using Hpredeclared. solve_into_val_typed. Qed.
+Proof. solve_into_val_typed. Qed.
+Global Instance into_val_comparable_uint32 : IntoValComparable w32 go.uint32.
+Proof. constructor. apply go.comparable_ordered. repeat constructor. Qed.
 
 Global Instance into_val_typed_uint16 : IntoValTyped w16 go.uint16.
-Proof using Hpredeclared. solve_into_val_typed. Qed.
+Proof. solve_into_val_typed. Qed.
+Global Instance into_val_comparable_uint16 : IntoValComparable w16 go.uint16.
+Proof. constructor. apply go.comparable_ordered. repeat constructor. Qed.
 
 Global Instance into_val_typed_uint8 : IntoValTyped w8 go.uint8.
-Proof using Hpredeclared. solve_into_val_typed. Qed.
+Proof. solve_into_val_typed. Qed.
+Global Instance into_val_comparable_uint8 : IntoValComparable w8 go.uint8.
+Proof. constructor. apply go.comparable_ordered. repeat constructor. Qed.
 
 Global Instance into_val_typed_uint : IntoValTyped w64 go.uint.
-Proof using Hpredeclared. solve_into_val_typed. Qed.
+Proof. solve_into_val_typed. Qed.
+Global Instance into_val_comparable_uint : IntoValComparable w64 go.uint.
+Proof. constructor. apply go.comparable_ordered. repeat constructor. Qed.
 
 Global Instance into_val_typed_int64 : IntoValTyped w64 go.int64.
-Proof using Hpredeclared. solve_into_val_typed. Qed.
+Proof. solve_into_val_typed. Qed.
+Global Instance into_val_comparable_int64 : IntoValComparable w64 go.int64.
+Proof. constructor. apply go.comparable_ordered. repeat constructor. Qed.
 
 Global Instance into_val_typed_int32 : IntoValTyped w32 go.int32.
-Proof using Hpredeclared. solve_into_val_typed. Qed.
+Proof. solve_into_val_typed. Qed.
+Global Instance into_val_comparable_int32 : IntoValComparable w32 go.int32.
+Proof. constructor. apply go.comparable_ordered. repeat constructor. Qed.
 
 Global Instance into_val_typed_int16 : IntoValTyped w16 go.int16.
-Proof using Hpredeclared. solve_into_val_typed. Qed.
+Proof. solve_into_val_typed. Qed.
+Global Instance into_val_comparable_int16 : IntoValComparable w16 go.int16.
+Proof. constructor. apply go.comparable_ordered. repeat constructor. Qed.
 
 Global Instance into_val_typed_int8 : IntoValTyped w8 go.int8.
-Proof using Hpredeclared. solve_into_val_typed. Qed.
+Proof. solve_into_val_typed. Qed.
+Global Instance into_val_comparable_int8 : IntoValComparable w8 go.int8.
+Proof. constructor. apply go.comparable_ordered. repeat constructor. Qed.
 
 Global Instance into_val_typed_int : IntoValTyped w64 go.int.
-Proof using Hpredeclared. solve_into_val_typed. Qed.
+Proof. solve_into_val_typed. Qed.
+Global Instance into_val_comparable_int : IntoValComparable w64 go.int.
+Proof. constructor. apply go.comparable_ordered. repeat constructor. Qed.
 
 Global Instance into_val_typed_bool : IntoValTyped bool go.bool.
-Proof using Hpredeclared. solve_into_val_typed. Qed.
+Proof. solve_into_val_typed. Qed.
+Global Instance into_val_comparable_bool : IntoValComparable bool go.bool.
+Proof. constructor. apply go.comparable_bool. Qed.
 
 Global Instance into_val_typed_string : IntoValTyped go_string go.string.
-Proof using Hpredeclared. solve_into_val_typed. Qed.
-
-Lemma seqZ_succ start n :
-  0 ≤ n →
-  seqZ start (Z.succ n) = seqZ start n ++ [start + n].
-Proof.
-  intros H. rewrite /seqZ Z2Nat.inj_succ; last lia.
-  rewrite seq_S fmap_app /=. f_equal. f_equal. lia.
-Qed.
+Proof. solve_into_val_typed. Qed.
+Global Instance into_val_comparable_string : IntoValComparable go_string go.string.
+Proof. constructor. apply go.comparable_ordered. repeat constructor. Qed.
 
 End into_val_typed_instances.
+
+Section inequality_instances.
+Context `{sem: ffi_semantics} `{!ffi_interp ffi} `{!heapGS Σ}
+  {Hcore : go.CoreSemantics} {Hpredeclared : go.PredeclaredSemantics}.
+
+Ltac solve_ineq lem :=
+  iIntros (?) "* _ * HΦ";
+  iApply wp_GoInstruction; [intros; repeat econstructor|];
+  iNext; iIntros "* %Hstep"; inv Hstep; inv Hpure;
+  iIntros "? $ !>"; rewrite lem; iApply "HΦ"; iFrame.
+
+Global Instance wp_le_uint (v1 v2 : w64) :
+  PureWp True (GoLe go.uint (#v1, #v2)%V) #(bool_decide (uint.Z v1 ≤ uint.Z v2)).
+Proof. solve_ineq go.le_uint. Qed.
+Global Instance wp_lt_uint (v1 v2 : w64) :
+  PureWp True (GoLt go.uint (#v1, #v2)%V) #(bool_decide (uint.Z v1 < uint.Z v2)).
+Proof. solve_ineq go.lt_uint. Qed.
+Global Instance wp_ge_uint (v1 v2 : w64) :
+  PureWp True (GoGe go.uint (#v1, #v2)%V) #(bool_decide (uint.Z v2 ≤ uint.Z v1)).
+Proof. solve_ineq go.le_uint. Qed.
+Global Instance wp_gt_uint (v1 v2 : w64) :
+  PureWp True (GoGt go.uint (#v1, #v2)%V) #(bool_decide (uint.Z v2 < uint.Z v1)).
+Proof. solve_ineq go.lt_uint. Qed.
+
+Global Instance wp_le_uint64 (v1 v2 : w64) :
+  PureWp True (GoLe go.uint64 (#v1, #v2)%V) #(bool_decide (uint.Z v1 ≤ uint.Z v2)).
+Proof. solve_ineq go.le_uint64. Qed.
+Global Instance wp_lt_uint64 (v1 v2 : w64) :
+  PureWp True (GoLt go.uint64 (#v1, #v2)%V) #(bool_decide (uint.Z v1 < uint.Z v2)).
+Proof. solve_ineq go.lt_uint64. Qed.
+Global Instance wp_ge_uint64 (v1 v2 : w64) :
+  PureWp True (GoGe go.uint64 (#v1, #v2)%V) #(bool_decide (uint.Z v2 ≤ uint.Z v1)).
+Proof. solve_ineq go.le_uint64. Qed.
+Global Instance wp_gt_uint64 (v1 v2 : w64) :
+  PureWp True (GoGt go.uint64 (#v1, #v2)%V) #(bool_decide (uint.Z v2 < uint.Z v1)).
+Proof. solve_ineq go.lt_uint64. Qed.
+
+Global Instance wp_le_uint32 (v1 v2 : w32) :
+  PureWp True (GoLe go.uint32 (#v1, #v2)%V) #(bool_decide (uint.Z v1 ≤ uint.Z v2)).
+Proof. solve_ineq go.le_uint32. Qed.
+Global Instance wp_lt_uint32 (v1 v2 : w32) :
+  PureWp True (GoLt go.uint32 (#v1, #v2)%V) #(bool_decide (uint.Z v1 < uint.Z v2)).
+Proof. solve_ineq go.lt_uint32. Qed.
+Global Instance wp_ge_uint32 (v1 v2 : w32) :
+  PureWp True (GoGe go.uint32 (#v1, #v2)%V) #(bool_decide (uint.Z v2 ≤ uint.Z v1)).
+Proof. solve_ineq go.le_uint32. Qed.
+Global Instance wp_gt_uint32 (v1 v2 : w32) :
+  PureWp True (GoGt go.uint32 (#v1, #v2)%V) #(bool_decide (uint.Z v2 < uint.Z v1)).
+Proof. solve_ineq go.lt_uint32. Qed.
+
+Global Instance wp_le_uint16 (v1 v2 : w16) :
+  PureWp True (GoLe go.uint16 (#v1, #v2)%V) #(bool_decide (uint.Z v1 ≤ uint.Z v2)).
+Proof. solve_ineq go.le_uint16. Qed.
+Global Instance wp_lt_uint16 (v1 v2 : w16) :
+  PureWp True (GoLt go.uint16 (#v1, #v2)%V) #(bool_decide (uint.Z v1 < uint.Z v2)).
+Proof. solve_ineq go.lt_uint16. Qed.
+Global Instance wp_ge_uint16 (v1 v2 : w16) :
+  PureWp True (GoGe go.uint16 (#v1, #v2)%V) #(bool_decide (uint.Z v2 ≤ uint.Z v1)).
+Proof. solve_ineq go.le_uint16. Qed.
+Global Instance wp_gt_uint16 (v1 v2 : w16) :
+  PureWp True (GoGt go.uint16 (#v1, #v2)%V) #(bool_decide (uint.Z v2 < uint.Z v1)).
+Proof. solve_ineq go.lt_uint16. Qed.
+
+Global Instance wp_le_uint8 (v1 v2 : w8) :
+  PureWp True (GoLe go.uint8 (#v1, #v2)%V) #(bool_decide (uint.Z v1 ≤ uint.Z v2)).
+Proof. solve_ineq go.le_uint8. Qed.
+Global Instance wp_lt_uint8 (v1 v2 : w8) :
+  PureWp True (GoLt go.uint8 (#v1, #v2)%V) #(bool_decide (uint.Z v1 < uint.Z v2)).
+Proof. solve_ineq go.lt_uint8. Qed.
+Global Instance wp_ge_uint8 (v1 v2 : w8) :
+  PureWp True (GoGe go.uint8 (#v1, #v2)%V) #(bool_decide (uint.Z v2 ≤ uint.Z v1)).
+Proof. solve_ineq go.le_uint8. Qed.
+Global Instance wp_gt_uint8 (v1 v2 : w8) :
+  PureWp True (GoGt go.uint8 (#v1, #v2)%V) #(bool_decide (uint.Z v2 < uint.Z v1)).
+Proof. solve_ineq go.lt_uint8. Qed.
+
+Global Instance wp_le_int (v1 v2 : w64) :
+  PureWp True (GoLe go.int (#v1, #v2)%V) #(bool_decide (sint.Z v1 ≤ sint.Z v2)).
+Proof. solve_ineq go.le_int. Qed.
+Global Instance wp_lt_int (v1 v2 : w64) :
+  PureWp True (GoLt go.int (#v1, #v2)%V) #(bool_decide (sint.Z v1 < sint.Z v2)).
+Proof. solve_ineq go.lt_int. Qed.
+Global Instance wp_ge_int (v1 v2 : w64) :
+  PureWp True (GoGe go.int (#v1, #v2)%V) #(bool_decide (sint.Z v2 ≤ sint.Z v1)).
+Proof. solve_ineq go.le_int. Qed.
+Global Instance wp_gt_int (v1 v2 : w64) :
+  PureWp True (GoGt go.int (#v1, #v2)%V) #(bool_decide (sint.Z v2 < sint.Z v1)).
+Proof. solve_ineq go.lt_int. Qed.
+
+Global Instance wp_le_int64 (v1 v2 : w64) :
+  PureWp True (GoLe go.int64 (#v1, #v2)%V) #(bool_decide (sint.Z v1 ≤ sint.Z v2)).
+Proof. solve_ineq go.le_int64. Qed.
+Global Instance wp_lt_int64 (v1 v2 : w64) :
+  PureWp True (GoLt go.int64 (#v1, #v2)%V) #(bool_decide (sint.Z v1 < sint.Z v2)).
+Proof. solve_ineq go.lt_int64. Qed.
+Global Instance wp_ge_int64 (v1 v2 : w64) :
+  PureWp True (GoGe go.int64 (#v1, #v2)%V) #(bool_decide (sint.Z v2 ≤ sint.Z v1)).
+Proof. solve_ineq go.le_int64. Qed.
+Global Instance wp_gt_int64 (v1 v2 : w64) :
+  PureWp True (GoGt go.int64 (#v1, #v2)%V) #(bool_decide (sint.Z v2 < sint.Z v1)).
+Proof. solve_ineq go.lt_int64. Qed.
+
+Global Instance wp_le_int32 (v1 v2 : w32) :
+  PureWp True (GoLe go.int32 (#v1, #v2)%V) #(bool_decide (sint.Z v1 ≤ sint.Z v2)).
+Proof. solve_ineq go.le_int32. Qed.
+Global Instance wp_lt_int32 (v1 v2 : w32) :
+  PureWp True (GoLt go.int32 (#v1, #v2)%V) #(bool_decide (sint.Z v1 < sint.Z v2)).
+Proof. solve_ineq go.lt_int32. Qed.
+Global Instance wp_ge_int32 (v1 v2 : w32) :
+  PureWp True (GoGe go.int32 (#v1, #v2)%V) #(bool_decide (sint.Z v2 ≤ sint.Z v1)).
+Proof. solve_ineq go.le_int32. Qed.
+Global Instance wp_gt_int32 (v1 v2 : w32) :
+  PureWp True (GoGt go.int32 (#v1, #v2)%V) #(bool_decide (sint.Z v2 < sint.Z v1)).
+Proof. solve_ineq go.lt_int32. Qed.
+
+Global Instance wp_le_int16 (v1 v2 : w16) :
+  PureWp True (GoLe go.int16 (#v1, #v2)%V) #(bool_decide (sint.Z v1 ≤ sint.Z v2)).
+Proof. solve_ineq go.le_int16. Qed.
+Global Instance wp_lt_int16 (v1 v2 : w16) :
+  PureWp True (GoLt go.int16 (#v1, #v2)%V) #(bool_decide (sint.Z v1 < sint.Z v2)).
+Proof. solve_ineq go.lt_int16. Qed.
+Global Instance wp_ge_int16 (v1 v2 : w16) :
+  PureWp True (GoGe go.int16 (#v1, #v2)%V) #(bool_decide (sint.Z v2 ≤ sint.Z v1)).
+Proof. solve_ineq go.le_int16. Qed.
+Global Instance wp_gt_int16 (v1 v2 : w16) :
+  PureWp True (GoGt go.int16 (#v1, #v2)%V) #(bool_decide (sint.Z v2 < sint.Z v1)).
+Proof. solve_ineq go.lt_int16. Qed.
+
+Global Instance wp_le_int8 (v1 v2 : w8) :
+  PureWp True (GoLe go.int8 (#v1, #v2)%V) #(bool_decide (sint.Z v1 ≤ sint.Z v2)).
+Proof. solve_ineq go.le_int8. Qed.
+Global Instance wp_lt_int8 (v1 v2 : w8) :
+  PureWp True (GoLt go.int8 (#v1, #v2)%V) #(bool_decide (sint.Z v1 < sint.Z v2)).
+Proof. solve_ineq go.lt_int8. Qed.
+Global Instance wp_ge_int8 (v1 v2 : w8) :
+  PureWp True (GoGe go.int8 (#v1, #v2)%V) #(bool_decide (sint.Z v2 ≤ sint.Z v1)).
+Proof. solve_ineq go.le_int8. Qed.
+Global Instance wp_gt_int8 (v1 v2 : w8) :
+  PureWp True (GoGt go.int8 (#v1, #v2)%V) #(bool_decide (sint.Z v2 < sint.Z v1)).
+Proof. solve_ineq go.lt_int8. Qed.
+
+End inequality_instances.
 
 Section __struct_test.
 Context `{sem: ffi_semantics} `{!ffi_interp ffi} `{!heapGS Σ}
